proof/correctness/Correctness_XMSS.ec
@@ -3,9 +3,15 @@ pragma Goals : printall.
 require import AllCore List RealExp IntDiv.
 from Jasmin require import JModel JArray.
 
-require import Params Parameters Address Notation Primitives Wots.
-require import XMSS_IMPL XMSS_IMPL_PP.
+require import Params Parameters Address Notation Primitives Wots XMSS_MT_PRF.
+require import XMSS_IMPL XMSS_IMPL_HOP1 RandomBytes.
 
+require import Array8 Array32 Array64.
 
+(*** Randomized Hashing ***)
+lemma thash_correct (_in : W8.t Array64.t,
+                     _pub_seed : W8.t Array32.t, 
+                     _addr:W32.t Array8.t) :
+    equiv[M_Hop1(Syscall).__thash_h ~ RandHash.rand_hash : true ==> true].
 
 (******* exported functions ********)
